test/Tests.lean
@@ -14,7 +14,9 @@ import Tests.Postmark
 import Tests.Postgres
 import Tests.RateLimit
 import Tests.Response
+import Tests.Session
 import Tests.Ses
 import Tests.Signup
 import Tests.Sql
+import Tests.Suppression
 import Tests.Template
